@prefix : <http://www.semanticweb.org/ontologies/2024/YOUTH#> .
@prefix owl: <http://www.w3.org/2002/07/owl#> .
@prefix rdf: <http://www.w3.org/1999/02/22-rdf-syntax-ns#> .
@prefix xml: <http://www.w3.org/XML/1998/namespace> .
@prefix xsd: <http://www.w3.org/2001/XMLSchema#> .
@prefix rdfs: <http://www.w3.org/2000/01/rdf-schema#> .
@prefix persp: <http://www.ontologydesignpatterns.org/ont/persp/perspectivisation.owl#> .
@prefix youth: <http://www.semanticweb.org/ontologies/2024/YOUTH/> .
@base <http://www.semanticweb.org/ontologies/2024/YOUTH#> .

<http://www.semanticweb.org/ontologies/2024/YOUTH> rdf:type owl:Ontology ;
                                                    owl:imports <http://www.ontologydesignpatterns.org/ont/persp/perspectivisation.owl> ;
                                                    <http://purl.org/dc/elements/1.1/creator> "Lucrezia Pograri" ,
                                                                                              "Pietro Tisci" ;
                                                    <http://purl.org/dc/elements/1.1/date> "August 2024" ;
                                                    rdfs:comment """YOUTH ontology was developed to interpret and describe the societal phenomenon of youth subcultures, including their members, historical context, and associated cultural practices, drawing on precise theoretical assumptions.

It is part of the end-of-course project of Knowledge Representation and Knowledge Extraction, taught by Professor Aldo Gangemi during the a.y. 2023/2024 at the University of Bologna, part of the Master’s program in Digital Humanities and Digital Knowledge.""" ;
                                                    rdfs:seeAlso "https://krke24.gitbook.io/krke-project-2023-2024" .

#################################################################
#    Object Properties
#################################################################

###  http://www.semanticweb.org/ontologies/2024/YOUTH#expressedVia
:expressedVia rdf:type owl:ObjectProperty ;
              rdfs:domain [ rdf:type owl:Class ;
                            owl:unionOf ( :NegativeAttitude
                                          :NeutralAttitude
                                          :PositiveAttitude
                                        )
                          ] ;
              rdfs:range [ rdf:type owl:Class ;
                           owl:unionOf ( youth:Stereotype
                                         youth:Value
                                       )
                         ] ;
              rdfs:comment "Links the classes Stereotype and Value to the classes PositiveAttitude, NegativeAttitude, and NeutralAttitude. It indicates that attitudes (positive, negative, or neutral) towards a subculture are shaped by the stereotypes associated with it and the values it upholds." .


###  http://www.semanticweb.org/ontologies/2024/YOUTH#fromExternalViewpointToAttitude
:fromExternalViewpointToAttitude rdf:type owl:ObjectProperty ;
                                 rdfs:subPropertyOf owl:topObjectProperty ;
                                 rdfs:domain youth:ExternalViewpoint ;
                                 rdfs:range [ rdf:type owl:Class ;
                                              owl:unionOf ( :NegativeAttitude
                                                            :NeutralAttitude
                                                            :PositiveAttitude
                                                          )
                                            ] ;
                                 rdfs:comment """This property captures the potential positive or negative attitude an individual with an external viewpoint has towards a youth subculture.

Example query: \"Individuals over x years of age have a positive attitude towards x youth subcultures.\"""" .


###  http://www.semanticweb.org/ontologies/2024/YOUTH#hasAttitude
:hasAttitude rdf:type owl:ObjectProperty ;
             owl:inverseOf :isAttitudeOf ;
             rdfs:domain youth:Person ;
             rdfs:range [ rdf:type owl:Class ;
                          owl:unionOf ( :NegativeAttitude
                                        :NeutralAttitude
                                        :PositiveAttitude
                                      )
                        ] .


###  http://www.semanticweb.org/ontologies/2024/YOUTH#hasRitual
:hasRitual rdf:type owl:ObjectProperty ;
           rdfs:domain youth:YouthSubculture ;
           rdfs:range youth:Ritual .


###  http://www.semanticweb.org/ontologies/2024/YOUTH#isAttitudeOf
:isAttitudeOf rdf:type owl:ObjectProperty ;
              rdfs:domain [ rdf:type owl:Class ;
                            owl:unionOf ( :NegativeAttitude
                                          :NeutralAttitude
                                          :PositiveAttitude
                                        )
                          ] ;
              rdfs:range youth:Person .


###  http://www.semanticweb.org/ontologies/2024/YOUTH#isViewpointOf
:isViewpointOf rdf:type owl:ObjectProperty ;
               owl:inverseOf youth:hasViewpoint ;
               rdfs:domain [ rdf:type owl:Class ;
                             owl:unionOf ( youth:ExternalViewpoint
                                           youth:InternalViewpoint
                                         )
                           ] ;
               rdfs:range youth:Person .


###  http://www.semanticweb.org/ontologies/2024/YOUTH/determinesShift
youth:determinesShift rdf:type owl:ObjectProperty ;
                      rdfs:domain [ rdf:type owl:Class ;
                                    owl:unionOf ( youth:ExternalViewpoint
                                                  youth:InternalViewpoint
                                                )
                                  ] ;
                      rdfs:range youth:PerspectiveShift ;
                      rdfs:comment "This property links a specific external or internal viewpoint to the perspective shift it determines. It captures how the views of subcultures, both internally (self-perception) and externally (public perception), are affected by shifts in perspective." .


###  http://www.semanticweb.org/ontologies/2024/YOUTH/hasFashionStyle
youth:hasFashionStyle rdf:type owl:ObjectProperty ;
                      rdfs:domain youth:YouthSubculture ;
                      rdfs:range youth:FashionStyle ;
                      rdfs:comment "Links a subculture to its fashion style(s)." .


###  http://www.semanticweb.org/ontologies/2024/YOUTH/hasMusicGenre
youth:hasMusicGenre rdf:type owl:ObjectProperty ;
                    rdfs:domain youth:YouthSubculture ;
                    rdfs:range youth:MusicGenre ;
                    rdfs:comment "Links a subculture to its associated music genre(s)." .


###  http://www.semanticweb.org/ontologies/2024/YOUTH/hasParticipant
youth:hasParticipant rdf:type owl:ObjectProperty ;
                     owl:inverseOf youth:participatesIn ;
                     rdfs:domain youth:YouthSubculture ;
                     rdfs:range youth:Person ;
                     rdfs:comment "Links a youth subculture to a person (indicating that the person is a member of the subculture)." .


###  http://www.semanticweb.org/ontologies/2024/YOUTH/hasValue
youth:hasValue rdf:type owl:ObjectProperty ;
               rdfs:domain youth:YouthSubculture ;
               rdfs:range youth:Value ;
               owl:propertyDisjointWith youth:triggersStereotype ;
               rdfs:comment "Links a subculture to its core values." .

[ rdf:type owl:Axiom ;
   owl:annotatedSource youth:hasValue ;
   owl:annotatedProperty owl:propertyDisjointWith ;
   owl:annotatedTarget youth:triggersStereotype ;
   rdfs:comment "Values and stereotypes have different implications."
 ] .


###  http://www.semanticweb.org/ontologies/2024/YOUTH/hasViewpoint
youth:hasViewpoint rdf:type owl:ObjectProperty ;
                   rdfs:domain youth:Person ;
                   rdfs:range [ rdf:type owl:Class ;
                                owl:unionOf ( youth:ExternalViewpoint
                                              youth:InternalViewpoint
                                            )
                              ] ;
                   rdfs:comment "Links a person to their internal or external viewpoint with regards to a youth subculture." .


###  http://www.semanticweb.org/ontologies/2024/YOUTH/influencedBy
youth:influencedBy rdf:type owl:ObjectProperty ;
                   rdfs:domain youth:ExternalViewpoint ,
                               youth:InternalViewpoint ;
                   rdfs:range youth:PerspectiveInfluence ;
                   rdfs:comment "Connects perspectives to the factors that influence them. This property shows how external and internal perspectives are affected by various influencing factors such as media representations, societal attitudes, and personal experiences. It models the relationship between perspectives and the elements that shape them." .


###  http://www.semanticweb.org/ontologies/2024/YOUTH/influences
youth:influences rdf:type owl:ObjectProperty ;
                 rdfs:subPropertyOf owl:topObjectProperty ;
                 rdfs:domain youth:YouthSubculture ;
                 rdfs:range youth:Person ,
                            youth:YouthSubculture ;
                 owl:propertyDisjointWith youth:triggersStereotype ;
                 rdfs:comment "Represents how a subculture influences the perspectives of individuals, itself, or other subcultures. This property models the impact that a subculture has on shaping the views and self-concepts of its members, its own evolution, as well as its influence on other subcultures" .

[ rdf:type owl:Axiom ;
   owl:annotatedSource youth:influences ;
   owl:annotatedProperty rdfs:comment ;
   owl:annotatedTarget "Represents how a subculture influences the perspectives of individuals, itself, or other subcultures. This property models the impact that a subculture has on shaping the views and self-concepts of its members, its own evolution, as well as its influence on other subcultures" ;
   rdfs:comment "Reflexive: a subculture can impact its own evolution and self-perception, not just its interactions with others. This self-influence reflects how subcultures continuously shape and reinforce their own identities, norms, and values from within, providing a more comprehensive and accurate representation of their internal dynamics."
 ] .


###  http://www.semanticweb.org/ontologies/2024/YOUTH/locatedIn
youth:locatedIn rdf:type owl:ObjectProperty ;
                rdfs:domain youth:YouthSubculture ;
                rdfs:range youth:Location ;
                rdfs:comment "Links individuals and subcultures to geographic locations." .


###  http://www.semanticweb.org/ontologies/2024/YOUTH/originatedIn
youth:originatedIn rdf:type owl:ObjectProperty ,
                            owl:FunctionalProperty ;
                   rdfs:domain youth:YouthSubculture ;
                   rdfs:range youth:HistoricalPeriod ;
                   rdfs:comment "Connects the youth subculture to its historical period, representing the time frame during which they have developed or undergone significant changes." .

[ rdf:type owl:Axiom ;
   owl:annotatedSource youth:originatedIn ;
   owl:annotatedProperty rdfs:comment ;
   owl:annotatedTarget "Connects the youth subculture to its historical period, representing the time frame during which they have developed or undergone significant changes." ;
   rdfs:comment "A subculture typically originates in one historical period, so this is a functional property."
 ] .


###  http://www.semanticweb.org/ontologies/2024/YOUTH/participatesIn
youth:participatesIn rdf:type owl:ObjectProperty ;
                     rdfs:domain youth:Person ;
                     rdfs:range youth:YouthSubculture ;
                     rdfs:comment "Links a Person to a YouthSubculture (indicating that the person belongs to that subculture)." .


###  http://www.semanticweb.org/ontologies/2024/YOUTH/triggersStereotype
youth:triggersStereotype rdf:type owl:ObjectProperty ;
                         rdfs:domain youth:YouthSubculture ;
                         rdfs:range youth:Stereotype ;
                         rdfs:comment "Links a stereotype to the subcultures that it affects or challenges. This property identifies how certain stereotypes are associated with subcultures and how these stereotypes may influence or be related to the subculture’s public image. It highlights the stereotypes that subcultures confront or embody." .


###  http://www.semanticweb.org/ontologies/2024/YOUTH/viewedAs
youth:viewedAs rdf:type owl:ObjectProperty ;
               rdfs:domain youth:YouthSubculture ;
               rdfs:range youth:ExternalViewpoint ;
               rdfs:comment "Links a youth subculture to its external viewpoint. This property connects subcultures to the way they are perceived by outsiders. It helps to model the public image and external characterization of a subculture." .


#################################################################
#    Data properties
#################################################################

###  http://www.semanticweb.org/ontologies/2024/YOUTH#belongsToGeneration
:belongsToGeneration rdf:type owl:DatatypeProperty ,
                              owl:FunctionalProperty ;
                     rdfs:range rdfs:Literal .


###  http://www.semanticweb.org/ontologies/2024/YOUTH/hasContext
youth:hasContext rdf:type owl:DatatypeProperty ;
                 rdfs:domain youth:HistoricalPeriod ;
                 rdfs:range rdfs:Literal ;
                 rdfs:comment "Describes the historical background in which a youth subculture originated." .


###  http://www.semanticweb.org/ontologies/2024/YOUTH/hasName
youth:hasName rdf:type owl:DatatypeProperty ,
                       owl:FunctionalProperty ;
              rdfs:domain youth:Person ;
              rdfs:range rdfs:Literal ;
              rdfs:comment "Indicates the name of a person." .


#################################################################
#    Classes
#################################################################

###  http://www.semanticweb.org/ontologies/2024/YOUTH#NegativeAttitude
:NegativeAttitude rdf:type owl:Class ;
                  rdfs:subClassOf persp:Attitude ,
                                  [ rdf:type owl:Restriction ;
                                    owl:onProperty :expressedVia ;
                                    owl:someValuesFrom youth:Stereotype
                                  ] ;
                  rdfs:comment "Attitude in this context refers to the evaluative stance or disposition that is held toward a youth subculture, whether by its members or by outsiders. Depending on whether a particular attitude aligns more closely with the values or stereotypes associated with a subculture, it will take on a positive, negative, or neutral connotation." .


###  http://www.semanticweb.org/ontologies/2024/YOUTH#NeutralAttitude
:NeutralAttitude rdf:type owl:Class ;
                 rdfs:subClassOf persp:Attitude ,
                                 [ rdf:type owl:Restriction ;
                                   owl:onProperty :expressedVia ;
                                   owl:someValuesFrom [ rdf:type owl:Class ;
                                                        owl:unionOf ( youth:Stereotype
                                                                      youth:Value
                                                                    )
                                                      ]
                                 ] ;
                 rdfs:comment "Attitude in this context refers to the evaluative stance or disposition that is held toward a youth subculture, whether by its members or by outsiders. Depending on whether a particular attitude aligns more closely with the values or stereotypes associated with a subculture, it will take on a positive, negative, or neutral connotation." .


###  http://www.semanticweb.org/ontologies/2024/YOUTH#PositiveAttitude
:PositiveAttitude rdf:type owl:Class ;
                  rdfs:subClassOf persp:Attitude ,
                                  [ rdf:type owl:Restriction ;
                                    owl:onProperty :expressedVia ;
                                    owl:someValuesFrom youth:Value
                                  ] ;
                  rdfs:comment "Attitude in this context refers to the evaluative stance or disposition that is held toward a youth subculture, whether by its members or by outsiders. Depending on whether a particular attitude aligns more closely with the values or stereotypes associated with a subculture, it will take on a positive, negative, or neutral connotation." .


###  http://www.semanticweb.org/ontologies/2024/YOUTH/ExternalViewpoint
youth:ExternalViewpoint rdf:type owl:Class ;
                        rdfs:subClassOf persp:Lens ,
                                        [ rdf:type owl:Restriction ;
                                          owl:onProperty :fromExternalViewpointToAttitude ;
                                          owl:someValuesFrom [ rdf:type owl:Class ;
                                                               owl:unionOf ( :NegativeAttitude
                                                                             :NeutralAttitude
                                                                             :PositiveAttitude
                                                                           )
                                                             ]
                                        ] ,
                                        [ rdf:type owl:Restriction ;
                                          owl:onProperty youth:influencedBy ;
                                          owl:someValuesFrom persp:Attitude
                                        ] ;
                        owl:disjointWith youth:InternalViewpoint ;
                        rdfs:comment "Represents the way in which subcultures are viewed from an external viewpoint. This is influenced by the general public's impressions, stereotypes, and media portrayals that shape the external image of a subculture." .


###  http://www.semanticweb.org/ontologies/2024/YOUTH/FashionStyle
youth:FashionStyle rdf:type owl:Class ;
                   rdfs:subClassOf youth:Style ,
                                   [ rdf:type owl:Restriction ;
                                     owl:onProperty youth:hasFashionStyle ;
                                     owl:someValuesFrom youth:Style
                                   ] ;
                   owl:disjointWith youth:MusicGenre ;
                   rdfs:comment "Represents the style of clothing and aesthetics associated with a subculture." .


###  http://www.semanticweb.org/ontologies/2024/YOUTH/HistoricalPeriod
youth:HistoricalPeriod rdf:type owl:Class ;
                       owl:disjointWith youth:Location ;
                       rdfs:comment "Represents the time frame (time-span) during which a subculture emerged, developed, or experienced significant influences." .


###  http://www.semanticweb.org/ontologies/2024/YOUTH/InternalViewpoint
youth:InternalViewpoint rdf:type owl:Class ;
                        rdfs:subClassOf persp:Lens ,
                                        [ rdf:type owl:Restriction ;
                                          owl:onProperty youth:influencedBy ;
                                          owl:someValuesFrom persp:Attitude
                                        ] ,
                                        [ rdf:type owl:Restriction ;
                                          owl:onProperty youth:influencedBy ;
                                          owl:someValuesFrom youth:PerspectiveInfluence
                                        ] ;
                        rdfs:comment "Represents the self-perception and self-definition of members within a subculture. This includes how individuals within the subculture view themselves and their own identity, as well as how they interpret their place within the subculture. It reflects the internal self-concept and personal narratives that members use to describe their experiences and values." .


###  http://www.semanticweb.org/ontologies/2024/YOUTH/Location
youth:Location rdf:type owl:Class ;
               rdfs:comment "This class defines the geographic context or physical setting where a subculture originates, encompassing specific regions, cities, or areas integral to its identity and activities. In the context of our project, \"location\" primarily refers to the geographical place (such as a city or state) where youth subcultures historically emerged. This meaning could be broadened to include more nuanced relationships, highlighting areas where these subcultures actively thrive or are predominantly practiced." .


###  http://www.semanticweb.org/ontologies/2024/YOUTH/MusicGenre
youth:MusicGenre rdf:type owl:Class ;
                 rdfs:subClassOf youth:Style ,
                                 [ rdf:type owl:Restriction ;
                                   owl:onProperty youth:hasMusicGenre ;
                                   owl:someValuesFrom youth:Style
                                 ] ;
                 rdfs:comment "Represents the type of music associated with a subculture." .


###  http://www.semanticweb.org/ontologies/2024/YOUTH/Person
youth:Person rdf:type owl:Class ;
             rdfs:subClassOf [ rdf:type owl:Restriction ;
                               owl:onProperty :hasAttitude ;
                               owl:someValuesFrom [ rdf:type owl:Class ;
                                                    owl:unionOf ( :NegativeAttitude
                                                                  :NeutralAttitude
                                                                  :PositiveAttitude
                                                                )
                                                  ]
                             ] ,
                             [ rdf:type owl:Restriction ;
                               owl:onProperty youth:hasViewpoint ;
                               owl:someValuesFrom [ rdf:type owl:Class ;
                                                    owl:unionOf ( youth:ExternalViewpoint
                                                                  youth:InternalViewpoint
                                                                )
                                                  ]
                             ] ,
                             [ rdf:type owl:Restriction ;
                               owl:onProperty youth:participatesIn ;
                               owl:someValuesFrom youth:YouthSubculture
                             ] ;
             owl:hasKey ( youth:hasName
                        ) ;
             rdfs:comment "Members within the youth subcultures." .


###  http://www.semanticweb.org/ontologies/2024/YOUTH/PerspectiveInfluence
youth:PerspectiveInfluence rdf:type owl:Class ;
                           rdfs:subClassOf persp:Background ;
                           owl:disjointWith youth:PerspectiveShift ;
                           rdfs:comment """Represents the factors that shape and affect both external and internal perspectives. This can include a variety of influences such as media portrayals, social institutions - like family, work, school, home -, personal experiences, education level, and cultural trends, all of which contribute to the evolving perceptions of subcultures by both insiders and outsiders. Hall’s Encoding/Decoding theory is integrated into this analysis, allowing us to deconstruct the role of television as a primary source of information on the subject.

See bibliography:
Hall, Stuart. \"Encoding/Decoding in the Television Discourse.\" University of Birmingham: Centre for Contemporary Cultural Studies, 1973.
Moore, Ryan. \"Alternative to What? Subcultural Capital and the Commercialization of a Music Scene.\" Deviant Behavior 26, no. 3 (2005): 229-252.""" .


###  http://www.semanticweb.org/ontologies/2024/YOUTH/PerspectiveShift
youth:PerspectiveShift rdf:type owl:Class ;
                       rdfs:subClassOf persp:Cut ,
                                       [ rdf:type owl:Restriction ;
                                         owl:onProperty youth:determinesShift ;
                                         owl:someValuesFrom [ rdf:type owl:Class ;
                                                              owl:unionOf ( youth:ExternalViewpoint
                                                                            youth:InternalViewpoint
                                                                          )
                                                            ]
                                       ] ;
                       rdfs:comment "Represents the interpretations or portrayals of a youth subculture following the evolution or transformation of perspectives. This class captures shifts in how subcultures are viewed, whether by the public or by their own members. It includes changes in societal attitudes, evolving stereotypes, or shifts in self-perception within the subculture, highlighting how perspectives can develop and alter across different historical or cultural contexts." .


###  http://www.semanticweb.org/ontologies/2024/YOUTH/Ritual
youth:Ritual rdf:type owl:Class ;
             rdfs:subClassOf youth:Style ,
                             [ rdf:type owl:Restriction ;
                               owl:onProperty :hasRitual ;
                               owl:someValuesFrom youth:Style
                             ] ;
             owl:disjointWith youth:Value ;
             rdfs:comment "Represents the activities that usually characterize a specific youth subculture." .


###  http://www.semanticweb.org/ontologies/2024/YOUTH/Stereotype
youth:Stereotype rdf:type owl:Class ;
                 rdfs:subClassOf [ rdf:type owl:Restriction ;
                                   owl:onProperty youth:triggersStereotype ;
                                   owl:someValuesFrom youth:YouthSubculture
                                 ] ;
                 owl:disjointWith youth:Value ;
                 rdfs:comment """Represents common stereotypes associated with subcultures, drawing on M. Cardwell's definition of a stereotype as \"a fixed, often simplistic generalization about a particular group or class of people. [...] These stereotypes are often negative and unflattering, and may underly prejudice and discrimination\". In our ontology, the Stereotype class encapsulates the generalized beliefs and oversimplified notions frequently attributed to members of specific subcultures. These stereotypes reflect societal perceptions and can shape mainstream discourse, influencing how subcultures are understood and portrayed. By capturing these stereotypes, the class facilitates the analysis of misrepresentations and biases that may skew public perception, offering insights into the disparity between societal views of subcultures and their actual characteristics and values.

See also:
Cardwell, Mike, Dictionary of Psychology, Chicago Fitzroy Dearborn, 1999: 292.""" .


###  http://www.semanticweb.org/ontologies/2024/YOUTH/Style
youth:Style rdf:type owl:Class ;
            owl:disjointWith youth:YouthSubculture ;
            rdfs:comment "Represents the overall style associated with a subculture, which can be further divided into Fashion Style, Music Genre, Ritual." .


###  http://www.semanticweb.org/ontologies/2024/YOUTH/Value
youth:Value rdf:type owl:Class ;
            rdfs:comment "Represents the fundamental principles and beliefs that underpin a subculture, guiding the behavior, attitudes, and norms of its members." .


###  http://www.semanticweb.org/ontologies/2024/YOUTH/YouthSubculture
youth:YouthSubculture rdf:type owl:Class ;
                      rdfs:subClassOf persp:Eventuality ,
                                      [ owl:intersectionOf ( [ rdf:type owl:Restriction ;
                                                               owl:onProperty :hasRitual ;
                                                               owl:someValuesFrom youth:Ritual
                                                             ]
                                                             [ rdf:type owl:Restriction ;
                                                               owl:onProperty youth:hasFashionStyle ;
                                                               owl:someValuesFrom youth:FashionStyle
                                                             ]
                                                             [ rdf:type owl:Restriction ;
                                                               owl:onProperty youth:hasMusicGenre ;
                                                               owl:someValuesFrom youth:MusicGenre
                                                             ]
                                                           ) ;
                                        rdf:type owl:Class
                                      ] ,
                                      [ rdf:type owl:Restriction ;
                                        owl:onProperty youth:hasParticipant ;
                                        owl:someValuesFrom youth:Person
                                      ] ,
                                      [ rdf:type owl:Restriction ;
                                        owl:onProperty youth:locatedIn ;
                                        owl:someValuesFrom youth:Location
                                      ] ,
                                      [ rdf:type owl:Restriction ;
                                        owl:onProperty youth:originatedIn ;
                                        owl:someValuesFrom youth:HistoricalPeriod
                                      ] ,
                                      [ rdf:type owl:Restriction ;
                                        owl:onProperty youth:viewedAs ;
                                        owl:someValuesFrom youth:ExternalViewpoint
                                      ] ,
                                      _:genid76 ;
                      rdfs:comment """A group of people within a cultural society that represents a specific community formed by younger generations, characterized by distinct values, practices, and identities that differentiate them from the dominant culture.

See bibliography:
Cohen, Albert K. Delinquent Boys: The Culture of the Gang. New York: Free Press, 1955.
Cohen, Phil. \"Subcultural Conflict and Working-Class Community.\" In CCCS Selected Working Papers, edited by Ann Gray, Jan Campbell, and Mark Erickson, 554-577. London: Routledge, 2007.
Williams, Patrick J. \"Youth Subcultural Studies: Sociological Traditions and Core Concepts.\" Sociology Compass 1, no. 2 (2007): 572-593.
Widdicombe, Sue. \"Autobiography and Change: Rhetoric and Authenticity of 'Gothic' Style.\" In Repertoires and Readings of Texts in Action, edited by Erica Burman and Ian Parker, 94-113. London: Routledge, 1993.""" ;
                      rdfs:seeAlso "https://krke24.gitbook.io/krke-project-2023-2024" .

_:genid76 rdf:type owl:Restriction ;
           owl:onProperty youth:influences ;
           owl:hasSelf "true"^^xsd:boolean .

[ rdf:type owl:Axiom ;
   owl:annotatedSource youth:YouthSubculture ;
   owl:annotatedProperty rdfs:subClassOf ;
   owl:annotatedTarget _:genid76 ;
   rdfs:comment "A youth subculture could potentially influence itself, but it's not necessarily always the case. Hence, the \"influences\" property is \"potentially reflexive\"."
 ] .


#################################################################
#    Annotations
#################################################################

owl:Thing <http://purl.org/dc/elements/1.1/creator> "Lucrezia Pograri" ,
                                                    "Pietro Tisci" ;
          <http://purl.org/dc/elements/1.1/date> 2024 ;
          rdfs:comment """YOUTH ontology interprets and describes the societal phenomenon of youth subcultures, including their members, historical context, and associated cultural practices, drawing on precise theoretical assumptions. 

It was developed as the end-of-the-course project of Knowledge Representation and Knowledge Extraction held by professor Aldo Gangemi in a.y. 2023/2024, Digital Humanities and Digital Knowledge - University of Bologna.

For further information, visit the following address:
https://krke24.gitbook.io/krke-project-2023-2024""" ;
          rdfs:seeAlso "https://krke24.gitbook.io/krke-project-2023-2024/methodology" .


###  Generated by the OWL API (version 4.5.29.2024-05-13T12:11:03Z) https://github.com/owlcs/owlapi
